Weidenbach_Book/IsaSAT_with_Restart.thy
@@ -729,7 +729,7 @@ proof -
     using 1 is_\<L>\<^sub>a\<^sub>l\<^sub>l_extract_atms_clss isasat_input_ops.is_\<L>\<^sub>a\<^sub>l\<^sub>l_def by auto
   finally show ?thesis .
 qed
-find_theorems mset_set image_mset image
+
 lemma cdcl\<^sub>W_ex_cdcl\<^sub>W_stgy:
   \<open>cdcl\<^sub>W_restart_mset.cdcl\<^sub>W S T \<Longrightarrow> \<exists>U. cdcl\<^sub>W_restart_mset.cdcl\<^sub>W_stgy S U\<close>
   by (meson cdcl\<^sub>W_restart_mset.cdcl\<^sub>W.cases cdcl\<^sub>W_restart_mset.cdcl\<^sub>W_stgy.simps)
